Adopted up to normalized zone semantics

Normalized_Zone_Semantics.thy
@@ -10,13 +10,13 @@ subsection \<open>Single Step\<close>
 
 inductive step_z_norm ::
   "('a, 'c, t, 's) ta
-  \<Rightarrow> 's \<Rightarrow> t DBM \<Rightarrow> (nat \<Rightarrow> nat) \<Rightarrow> ('c \<Rightarrow> nat) \<Rightarrow> nat \<Rightarrow> 'a action \<Rightarrow> 's \<Rightarrow> t DBM \<Rightarrow> bool"
+  \<Rightarrow> 's \<Rightarrow> t DBM \<Rightarrow> ('s \<Rightarrow> nat \<Rightarrow> nat) \<Rightarrow> ('c \<Rightarrow> nat) \<Rightarrow> nat \<Rightarrow> 'a action \<Rightarrow> 's \<Rightarrow> t DBM \<Rightarrow> bool"
 ("_ \<turnstile> \<langle>_, _\<rangle> \<leadsto>\<^bsub>_,_,_,_\<^esub> \<langle>_, _\<rangle>" [61,61,61,61,61,61] 61)
 where step_z_norm:
-  "A \<turnstile> \<langle>l,D\<rangle> \<leadsto>\<^bsub>v,n,a\<^esub> \<langle>l', D'\<rangle> \<Longrightarrow> A \<turnstile> \<langle>l,D\<rangle> \<leadsto>\<^bsub>k,v,n,a\<^esub> \<langle>l', norm (FW D' n) k n\<rangle>"
+  "A \<turnstile> \<langle>l,D\<rangle> \<leadsto>\<^bsub>v,n,a\<^esub> \<langle>l', D'\<rangle> \<Longrightarrow> A \<turnstile> \<langle>l,D\<rangle> \<leadsto>\<^bsub>k,v,n,a\<^esub> \<langle>l', norm (FW D' n) (k l') n\<rangle>"
 
 inductive steps_z_norm ::
-  "('a, 'c, t, 's) ta \<Rightarrow> 's \<Rightarrow> t DBM \<Rightarrow> (nat \<Rightarrow> nat) \<Rightarrow> ('c \<Rightarrow> nat) \<Rightarrow> nat \<Rightarrow> 's \<Rightarrow> t DBM \<Rightarrow> bool"
+  "('a, 'c, t, 's) ta \<Rightarrow> 's \<Rightarrow> t DBM \<Rightarrow> ('s \<Rightarrow> nat \<Rightarrow> nat) \<Rightarrow> ('c \<Rightarrow> nat) \<Rightarrow> nat \<Rightarrow> 's \<Rightarrow> t DBM \<Rightarrow> bool"
 ("_ \<turnstile> \<langle>_, _\<rangle> \<leadsto>\<^bsub>_,_,_\<^esub>* \<langle>_, _\<rangle>" [61,61,61,61,61] 61)
 where
   refl: "A \<turnstile> \<langle>l, Z\<rangle> \<leadsto>\<^bsub>k,v,n\<^esub>* \<langle>l, Z\<rangle>" |
@@ -40,28 +40,8 @@ lemma norm_empty_diag_preservation_real:
   shows "norm M (real o k) n i i < Le 0"
 using assms unfolding norm_def by (force simp: Let_def less dest: dbm_lt_trans)
 
-context Regions
+context Regions_defs
 begin
-
-abbreviation "v' \<equiv> beta_interp.v'"
-
-abbreviation step_z_norm' ("_ \<turnstile> \<langle>_, _\<rangle> \<leadsto>\<^bsub>\<N>(_)\<^esub> \<langle>_, _\<rangle>" [61,61,61,61] 61)
-where
-  "A \<turnstile> \<langle>l, D\<rangle> \<leadsto>\<^bsub>\<N>(a)\<^esub> \<langle>l', D'\<rangle> \<equiv> A \<turnstile> \<langle>l, D\<rangle> \<leadsto>\<^bsub>(k o v'),v,n,a\<^esub> \<langle>l', D'\<rangle>"
-
-abbreviation steps_z_norm' ("_ \<turnstile> \<langle>_, _\<rangle> \<leadsto>\<^sub>\<N>* \<langle>_, _\<rangle>" [61,61,61] 61)
-where
-  "A \<turnstile> \<langle>l, D\<rangle> \<leadsto>\<^sub>\<N>* \<langle>l', D'\<rangle> \<equiv> A \<turnstile> \<langle>l, D\<rangle> \<leadsto>\<^bsub>(k o v'),v,n\<^esub>* \<langle>l', D'\<rangle>"
-
-inductive_cases[elim!]: "A \<turnstile> \<langle>l, u\<rangle> \<leadsto>\<^bsub>\<N>(a)\<^esub> \<langle>l',u'\<rangle>"
-
-declare step_z_norm.intros[intro]
-
-lemma apx_empty_iff'':
-  assumes "canonical M1 n" "[M1]\<^bsub>v,n\<^esub> \<subseteq> V" "dbm_int M1 n"
-  shows "[M1]\<^bsub>v,n\<^esub> = {} \<longleftrightarrow> [norm M1 (k o v') n]\<^bsub>v,n\<^esub> = {}"
-  using beta_interp.apx_norm_eq[OF assms] apx_empty_iff'[of "[M1]\<^bsub>v,n\<^esub>"] assms
-  unfolding V'_def by blast
 
 inductive valid_dbm where
   "[M]\<^bsub>v,n\<^esub> \<subseteq> V \<Longrightarrow> dbm_int M n \<Longrightarrow> valid_dbm M"
@@ -70,24 +50,21 @@ inductive_cases valid_dbm_cases[elim]: "valid_dbm M"
 
 declare valid_dbm.intros[intro]
 
-lemma step_z_valid_dbm:
-  assumes "A \<turnstile> \<langle>l, D\<rangle> \<leadsto>\<^bsub>v,n,a\<^esub> \<langle>l', D'\<rangle>"
-    and "global_clock_numbering A v n" "valid_abstraction A X k" "valid_dbm D"
-  shows "valid_dbm D'"
-proof -
-  from alpha_interp.step_z_V step_z_dbm_sound[OF assms(1,2)] step_z_dbm_preserves_int[OF assms(1,2)]
-       assms(3,4)
-  have
-    "dbm_int D' n" "A \<turnstile> \<langle>l, [D]\<^bsub>v,n\<^esub>\<rangle> \<leadsto>\<^bsub>a\<^esub> \<langle>l', [D']\<^bsub>v,n\<^esub>\<rangle>"
-  by fastforce+
-  with alpha_interp.step_z_V[OF this(2)] assms(4) show ?thesis by auto
-qed
+end (* End of context for augmenting definitions for local and global sets of regions *)
+
+locale Regions_common =
+  Regions_defs X v n for X :: "'c set" and v n +
+  fixes not_in_X
+  assumes finite: "finite X"
+  assumes clock_numbering: "clock_numbering' v n" "\<forall>k\<le>n. k > 0 \<longrightarrow> (\<exists>c \<in> X. v c = k)"
+                           "\<forall> c \<in> X. v c \<le> n"
+  assumes not_in_X: "not_in_X \<notin> X"
+  assumes non_empty: "X \<noteq> {}"
+begin
 
 lemma FW_zone_equiv_spec:
   shows "[M]\<^bsub>v,n\<^esub> = [FW M n]\<^bsub>v,n\<^esub>"
 apply (rule FW_zone_equiv) using clock_numbering(2) by auto
-
-lemma cn_weak: "\<forall>k\<le>n. 0 < k \<longrightarrow> (\<exists>c. v c = k)" using clock_numbering(2) by blast
 
 lemma dbm_non_empty_diag:
   assumes "[M]\<^bsub>v,n\<^esub> \<noteq> {}"
@@ -98,6 +75,8 @@ proof safe
   from k not_empty_cyc_free[OF this assms(1)] show "\<one> \<le> M k k" by (simp add: cyc_free_diag_dest')
 qed
 
+lemma cn_weak: "\<forall>k\<le>n. 0 < k \<longrightarrow> (\<exists>c. v c = k)" using clock_numbering(2) by blast
+
 lemma negative_diag_empty:
   assumes "\<exists> k \<le> n. M k k < \<one>"
   shows "[M]\<^bsub>v,n\<^esub> = {}"
@@ -107,6 +86,30 @@ lemma non_empty_cycle_free:
   assumes "[M]\<^bsub>v,n\<^esub> \<noteq> {}"
   shows "cycle_free M n"
 by (meson assms clock_numbering(2) neg_cycle_empty negative_cycle_dest_diag)
+
+lemma FW_valid_preservation:
+  assumes "valid_dbm M"
+  shows "valid_dbm (FW M n)"
+proof standard
+  from FW_int_preservation assms show "dbm_int (FW M n) n" by blast
+next
+  from FW_zone_equiv_spec[of M, folded neutral] assms show "[FW M n]\<^bsub>v,n\<^esub> \<subseteq> V" by fastforce
+qed
+
+end
+
+context Regions_global
+begin
+
+sublocale Regions_common by standard (rule finite clock_numbering not_in_X non_empty)+
+
+abbreviation "v' \<equiv> beta_interp.v'"
+
+lemma apx_empty_iff'':
+  assumes "canonical M1 n" "[M1]\<^bsub>v,n\<^esub> \<subseteq> V" "dbm_int M1 n"
+  shows "[M1]\<^bsub>v,n\<^esub> = {} \<longleftrightarrow> [norm M1 (k o v') n]\<^bsub>v,n\<^esub> = {}"
+  using beta_interp.apx_norm_eq[OF assms] apx_empty_iff'[of "[M1]\<^bsub>v,n\<^esub>"] assms
+  unfolding V'_def by blast
 
 lemma norm_FW_empty:
   assumes "valid_dbm M"
@@ -132,26 +135,6 @@ proof -
   with beta_interp.apx_norm_eq[OF fw_canonical[OF cyc_free] _ FW_int_preservation]
       dbm_non_empty_diag[OF assms(2)] assms(1)
  show "Approx\<^sub>\<beta> ([M]\<^bsub>v,n\<^esub>) = [norm (FW M n) (k o v') n]\<^bsub>v,n\<^esub>" by auto
-
-qed
-
-(* Crudely copied from step_z_norm.inducts *)
-lemma step_z_norm_induct[case_names _ step_z_norm step_z_refl]:
-  assumes "x1 \<turnstile> \<langle>x2, x3\<rangle> \<leadsto>\<^bsub>(k o v'),v,n,a\<^esub> \<langle>x7,x8\<rangle>"
-    and step_z_norm:
-    "\<And>A l D l' D'.
-        A \<turnstile> \<langle>l, D\<rangle> \<leadsto>\<^bsub>v,n,a\<^esub> \<langle>l',D'\<rangle> \<Longrightarrow>
-        P A l D l' (norm (FW D' n) (k o v') n)"
-  shows "P x1 x2 x3 x7 x8"
-using assms by (induction rule: step_z_norm.inducts) auto
-
-lemma FW_valid_preservation:
-  assumes "valid_dbm M"
-  shows "valid_dbm (FW M n)"
-proof standard
-  from FW_int_preservation assms show "dbm_int (FW M n) n" by blast
-next
-  from FW_zone_equiv_spec[of M, folded neutral] assms show "[FW M n]\<^bsub>v,n\<^esub> \<subseteq> V" by fastforce
 qed
 
 lemma norm_FW_valid_preservation_non_empty:
@@ -174,18 +157,6 @@ lemma norm_int_all_preservation:
   shows "dbm_int_all (norm M (k o v') n)"
 using assms unfolding norm_def by (auto simp: Let_def)
 
-lemma step_z_norm_int_all_preservation:
-  assumes
-    "A \<turnstile> \<langle>l,D\<rangle> \<leadsto>\<^bsub>\<N>(a)\<^esub> \<langle>l',D'\<rangle>" "global_clock_numbering A v n" "valid_abstraction A X k" "dbm_int_all D"
-  shows "dbm_int_all D'"
-using assms
- apply cases
- apply simp
- apply (rule norm_int_all_preservation[simplified])
- apply (rule FW_int_all_preservation)
- apply (erule step_z_dbm_preserves_int_all)
-by fast+
-
 lemma norm_FW_valid_preservation_empty:
   assumes "valid_dbm M" "[M]\<^bsub>v,n\<^esub> = {}"
   shows "valid_dbm (norm (FW M n) (k o v') n)" (is "valid_dbm ?M")
@@ -204,31 +175,124 @@ lemma norm_FW_valid_preservation:
   shows "valid_dbm (norm (FW M n) (k o v') n)"
 using assms norm_FW_valid_preservation_empty norm_FW_valid_preservation_non_empty by metis
 
+lemma norm_FW_equiv:
+  assumes valid: "dbm_int D n" "dbm_int M n" "[D]\<^bsub>v,n\<^esub> \<subseteq> V"
+      and equiv: "[D]\<^bsub>v,n\<^esub> = [M]\<^bsub>v,n\<^esub>"
+  shows "[norm (FW D n) (k o v') n]\<^bsub>v,n\<^esub> = [norm (FW M n) (k o v') n]\<^bsub>v,n\<^esub>"
+proof (cases "[D]\<^bsub>v,n\<^esub> = {}")
+  case False
+  with equiv fw_shortest local.non_empty_cycle_free FW_zone_equiv_spec have
+    "canonical (FW D n) n" "canonical (FW M n) n" "[FW D n]\<^bsub>v,n\<^esub> = [D]\<^bsub>v,n\<^esub>" "[FW M n]\<^bsub>v,n\<^esub> = [M]\<^bsub>v,n\<^esub>"
+  by blast+
+  with valid equiv show ?thesis
+   apply -
+   apply (subst beta_interp.apx_norm_eq[symmetric])
+   prefer 4
+   apply (subst beta_interp.apx_norm_eq[symmetric])
+  by (simp add: FW_int_preservation)+
+next
+  case True
+  show ?thesis
+   apply (subst norm_FW_empty)
+   prefer 3
+   apply (subst norm_FW_empty)
+  using valid equiv True by blast+
+qed
+
+end (* End of context for global set of regions *)
+
+context Regions
+begin
+
+sublocale Regions_common by standard (rule finite clock_numbering not_in_X non_empty)+
+
+definition "v' \<equiv> \<lambda> i. if 0 < i \<and> i \<le> n then (THE c. c \<in> X \<and> v c = i) else not_in_X"
+(*abbreviation "v' \<equiv> beta_interp.v'"*)
+
+abbreviation step_z_norm' ("_ \<turnstile> \<langle>_, _\<rangle> \<leadsto>\<^bsub>\<N>(_)\<^esub> \<langle>_, _\<rangle>" [61,61,61,61] 61)
+where
+  "A \<turnstile> \<langle>l, D\<rangle> \<leadsto>\<^bsub>\<N>(a)\<^esub> \<langle>l', D'\<rangle> \<equiv> A \<turnstile> \<langle>l, D\<rangle> \<leadsto>\<^bsub>(\<lambda> l. k l o v'),v,n,a\<^esub> \<langle>l', D'\<rangle>"
+
+abbreviation steps_z_norm' ("_ \<turnstile> \<langle>_, _\<rangle> \<leadsto>\<^sub>\<N>* \<langle>_, _\<rangle>" [61,61,61] 61)
+where
+  "A \<turnstile> \<langle>l, D\<rangle> \<leadsto>\<^sub>\<N>* \<langle>l', D'\<rangle> \<equiv> A \<turnstile> \<langle>l, D\<rangle> \<leadsto>\<^bsub>(\<lambda> l. k l o v'),v,n\<^esub>* \<langle>l', D'\<rangle>"
+
+inductive_cases[elim!]: "A \<turnstile> \<langle>l, u\<rangle> \<leadsto>\<^bsub>\<N>(a)\<^esub> \<langle>l',u'\<rangle>"
+
+declare step_z_norm.intros[intro]
+
+lemma step_z_valid_dbm:
+  assumes "A \<turnstile> \<langle>l, D\<rangle> \<leadsto>\<^bsub>v,n,a\<^esub> \<langle>l', D'\<rangle>"
+    and "global_clock_numbering A v n" "valid_abstraction A X k" "valid_dbm D"
+  shows "valid_dbm D'"
+proof -
+  from step_z_V step_z_dbm_sound[OF assms(1,2)] step_z_dbm_preserves_int[OF assms(1,2)]
+       assms(3,4)
+  have
+    "dbm_int D' n" "A \<turnstile> \<langle>l, [D]\<^bsub>v,n\<^esub>\<rangle> \<leadsto>\<^bsub>a\<^esub> \<langle>l', [D']\<^bsub>v,n\<^esub>\<rangle>"
+  by (fastforce dest!: valid_abstraction_pairsD)+
+  with step_z_V[OF this(2)] assms(4) show ?thesis by auto
+qed
+
+(* Crudely copied from step_z_norm.inducts *)
+lemma step_z_norm_induct[case_names _ step_z_norm step_z_refl]:
+  assumes "x1 \<turnstile> \<langle>x2, x3\<rangle> \<leadsto>\<^bsub>(\<lambda> l. k l o v'),v,n,a\<^esub> \<langle>x7,x8\<rangle>"
+    and step_z_norm:
+    "\<And>A l D l' D'.
+        A \<turnstile> \<langle>l, D\<rangle> \<leadsto>\<^bsub>v,n,a\<^esub> \<langle>l',D'\<rangle> \<Longrightarrow>
+        P A l D l' (norm (FW D' n) (k l' o v') n)"
+  shows "P x1 x2 x3 x7 x8"
+using assms by (induction rule: step_z_norm.inducts) auto
+
+context
+  fixes l' :: 's
+begin
+
+interpretation regions: Regions_global _ _ _ "k l'"
+  by standard (rule finite clock_numbering not_in_X non_empty)+
+
+lemma [simp]:
+  "regions.v' = v'"
+  unfolding v'_def regions.beta_interp.v'_def by simp
+
+lemma step_z_norm_int_all_preservation:
+  assumes
+    "A \<turnstile> \<langle>l,D\<rangle> \<leadsto>\<^bsub>\<N>(a)\<^esub> \<langle>l',D'\<rangle>" "global_clock_numbering A v n"
+    "\<forall>(x, m)\<in>Timed_Automata.clkp_set A. m \<in> \<nat>" "dbm_int_all D"
+  shows "dbm_int_all D'"
+using assms
+ apply cases
+ apply simp
+ apply (rule regions.norm_int_all_preservation[simplified])
+ apply (rule FW_int_all_preservation)
+ apply (erule step_z_dbm_preserves_int_all)
+by fast+
+
 lemma step_z_norm_valid_dbm_preservation:
   assumes
     "A \<turnstile> \<langle>l,D\<rangle> \<leadsto>\<^bsub>\<N>(a)\<^esub> \<langle>l',D'\<rangle>" "global_clock_numbering A v n" "valid_abstraction A X k" "valid_dbm D"
   shows "valid_dbm D'"
-using assms by cases (simp; rule norm_FW_valid_preservation[simplified]; erule step_z_valid_dbm; fast)
-
-
+  using assms
+  by cases (simp; rule regions.norm_FW_valid_preservation[simplified]; erule step_z_valid_dbm; fast)
 
 lemma norm_beta_sound:
   assumes "A \<turnstile> \<langle>l,D\<rangle> \<leadsto>\<^bsub>\<N>(a)\<^esub> \<langle>l',D'\<rangle>" "global_clock_numbering A v n" "valid_abstraction A X k"
   and     "valid_dbm D"
 shows   "A \<turnstile> \<langle>l,[D]\<^bsub>v,n\<^esub>\<rangle> \<leadsto>\<^bsub>\<beta>(a)\<^esub> \<langle>l',[D']\<^bsub>v,n\<^esub>\<rangle>" using assms(2-) thm step_z_norm_induct
-  apply (induction A l D l' D' rule: step_z_norm_induct, (subst assms(1); blast))
+  apply (induction A l D l' \<equiv> l' D' rule: step_z_norm_induct, (subst assms(1); blast))
 proof goal_cases
-  case step_z_norm: (1 A l D l' D')
+  case step_z_norm: (1 A l D D')
   from step_z_dbm_sound[OF step_z_norm(1,2)] have "A \<turnstile> \<langle>l, [D]\<^bsub>v,n\<^esub>\<rangle> \<leadsto>\<^bsub>a\<^esub> \<langle>l',[D']\<^bsub>v,n\<^esub>\<rangle>" by blast
-  then have *: "A \<turnstile> \<langle>l, [D]\<^bsub>v,n\<^esub>\<rangle> \<leadsto>\<^bsub>\<beta>(a)\<^esub> \<langle>l',Approx\<^sub>\<beta> ([D']\<^bsub>v,n\<^esub>)\<rangle>" by force
+  then have *: "A \<turnstile> \<langle>l, [D]\<^bsub>v,n\<^esub>\<rangle> \<leadsto>\<^bsub>\<beta>(a)\<^esub> \<langle>l',Approx\<^sub>\<beta> l' ([D']\<^bsub>v,n\<^esub>)\<rangle>" by force
   show ?case
   proof (cases "[D']\<^bsub>v,n\<^esub> = {}")
     case False
-    from apx_norm_eq_spec[OF step_z_valid_dbm[OF step_z_norm] False] *
+    from regions.apx_norm_eq_spec[OF step_z_valid_dbm[OF step_z_norm] False] *
     show ?thesis by auto
   next
     case True
-    with norm_FW_empty[OF step_z_valid_dbm[OF step_z_norm] this] beta_interp.apx_empty *
+    with
+      regions.norm_FW_empty[OF step_z_valid_dbm[OF step_z_norm] this] regions.beta_interp.apx_empty *
     show ?thesis by auto
   qed
 qed
@@ -238,10 +302,10 @@ lemma step_z_norm_valid_dbm:
     "A \<turnstile> \<langle>l, D\<rangle> \<leadsto>\<^bsub>\<N>(a)\<^esub> \<langle>l',D'\<rangle>" "global_clock_numbering A v n"
     "valid_abstraction A X k" "valid_dbm D"
   shows "valid_dbm D'" using assms(2-)
-apply (induction A l D l' D' rule: step_z_norm_induct, (subst assms(1); blast))
+apply (induction A l D l' \<equiv> l' D' rule: step_z_norm_induct, (subst assms(1); blast))
 proof goal_cases
-  case step_z_norm: (1 A l D l' D')
-  with norm_FW_valid_preservation[OF step_z_valid_dbm[OF step_z_norm]] show ?case by fast
+  case step_z_norm: (1 A l D D')
+  with regions.norm_FW_valid_preservation[OF step_z_valid_dbm[OF step_z_norm]] show ?case by auto
 qed
 
 lemma norm_beta_complete:
@@ -249,24 +313,30 @@ lemma norm_beta_complete:
   and     "valid_dbm D"
   obtains D' where "A \<turnstile> \<langle>l,D\<rangle> \<leadsto>\<^bsub>\<N>(a)\<^esub> \<langle>l',D'\<rangle>" "[D']\<^bsub>v,n\<^esub> = Z" "valid_dbm D'"
 proof -
-  from assms(1) obtain Z' where Z': "A \<turnstile> \<langle>l,[D]\<^bsub>v,n\<^esub>\<rangle> \<leadsto>\<^bsub>a\<^esub> \<langle>l',Z'\<rangle>" "Z = Approx\<^sub>\<beta> Z'" by auto
+  from assms(3) have ta_int: "\<forall>(x, m)\<in>Timed_Automata.clkp_set A. m \<in> \<nat>"
+    by (fastforce dest!: valid_abstraction_pairsD)
+  from assms(1) obtain Z' where Z': "A \<turnstile> \<langle>l,[D]\<^bsub>v,n\<^esub>\<rangle> \<leadsto>\<^bsub>a\<^esub> \<langle>l',Z'\<rangle>" "Z = Approx\<^sub>\<beta> l' Z'" by auto
   from assms(4) have "dbm_int D n" by auto
-  with step_z_dbm_DBM[OF Z'(1) assms(2)] step_z_dbm_preserves_int[OF _ assms(2,3)] obtain D' where
-    D': "A \<turnstile> \<langle>l, D\<rangle> \<leadsto>\<^bsub>v,n,a\<^esub> \<langle>l',D'\<rangle>" "Z' = [D']\<^bsub>v,n\<^esub>" "dbm_int D' n"
+  with step_z_dbm_DBM[OF Z'(1) assms(2)] step_z_dbm_preserves_int[OF _ assms(2) ta_int] obtain D'
+    where D': "A \<turnstile> \<langle>l, D\<rangle> \<leadsto>\<^bsub>v,n,a\<^esub> \<langle>l',D'\<rangle>" "Z' = [D']\<^bsub>v,n\<^esub>" "dbm_int D' n"
   by auto
   note valid_D' = step_z_valid_dbm[OF D'(1) assms(2,3)]
-  obtain D'' where D'': "D'' = norm (FW D' n) (k \<circ> v') n" by auto
+  obtain D'' where D'': "D'' = norm (FW D' n) (k l' \<circ> v') n" by auto
   show ?thesis
   proof (cases "Z' = {}")
     case False
     with D' have *: "[D']\<^bsub>v,n\<^esub> \<noteq> {}" by auto
-    from apx_norm_eq_spec[OF valid_D' this] D'' D'(2) Z'(2) assms(4) have "Z = [D'']\<^bsub>v,n\<^esub>" by auto
-    with norm_FW_valid_preservation[OF valid_D'] D' D'' * that[of D''] assms(4)
-    show thesis by blast
+    from regions.apx_norm_eq_spec[OF valid_D' this] D'' D'(2) Z'(2) assms(4) have "Z = [D'']\<^bsub>v,n\<^esub>"
+      by auto
+    with regions.norm_FW_valid_preservation[OF valid_D'] D' D'' *  assms(4)
+    show thesis
+      apply -
+      apply (rule that[of D''])
+      by (drule step_z_norm.intros[where k = "\<lambda> l. k l o v'"]) simp+
   next
     case True
-    with norm_FW_empty[OF valid_D'[OF assms(4)]] D'' D' Z'(2)
-         norm_FW_valid_preservation[OF valid_D'[OF assms(4)]] beta_interp.apx_empty
+    with regions.norm_FW_empty[OF valid_D'[OF assms(4)]] D'' D' Z'(2)
+         regions.norm_FW_valid_preservation[OF valid_D'[OF assms(4)]] regions.beta_interp.apx_empty
     show thesis
     apply -
     apply (rule that[of D''])
@@ -281,19 +351,51 @@ lemma norm_beta_empty:
   shows   "[D']\<^bsub>v,n\<^esub> = {}" using assms
 oops
 
+(* XXX Maybe move *)
+lemma step_z_norm_mono:
+  assumes "A \<turnstile> \<langle>l,D\<rangle> \<leadsto>\<^bsub>\<N>(a)\<^esub> \<langle>l',D'\<rangle>" "global_clock_numbering A v n" "valid_abstraction A X k"
+  and     "valid_dbm D" "valid_dbm M"
+  and "[D]\<^bsub>v,n\<^esub> \<subseteq> [M]\<^bsub>v,n\<^esub>"
+  shows "\<exists> M'. A \<turnstile> \<langle>l, M\<rangle> \<leadsto>\<^bsub>\<N>(a)\<^esub> \<langle>l', M'\<rangle> \<and> [D']\<^bsub>v,n\<^esub> \<subseteq> [M']\<^bsub>v,n\<^esub>"
+proof -
+  from norm_beta_sound[OF assms(1,2,3,4)] have "A \<turnstile> \<langle>l, [D]\<^bsub>v,n\<^esub>\<rangle> \<leadsto>\<^bsub>\<beta>(a)\<^esub> \<langle>l', [D']\<^bsub>v,n\<^esub>\<rangle>" .
+  from step_z_beta_mono[OF this assms(6)] assms(5) obtain Z where
+    "A \<turnstile> \<langle>l, [M]\<^bsub>v,n\<^esub>\<rangle> \<leadsto>\<^bsub>\<beta>(a)\<^esub> \<langle>l', Z\<rangle>" "[D']\<^bsub>v,n\<^esub> \<subseteq> Z"
+  by auto
+  with norm_beta_complete[OF this(1) assms(2,3,5)] show ?thesis by metis
+qed
+
+lemma step_z_norm_equiv:
+  assumes step: "A \<turnstile> \<langle>l,D\<rangle> \<leadsto>\<^bsub>\<N>(a)\<^esub> \<langle>l',D'\<rangle>"
+      and prems: "global_clock_numbering A v n" "valid_abstraction A X k"
+      and valid: "valid_dbm D" "valid_dbm M"
+      and equiv: "[D]\<^bsub>v,n\<^esub> = [M]\<^bsub>v,n\<^esub>"
+  shows "\<exists> M'. A \<turnstile> \<langle>l, M\<rangle> \<leadsto>\<^bsub>\<N>(a)\<^esub> \<langle>l', M'\<rangle> \<and> [D']\<^bsub>v,n\<^esub> = [M']\<^bsub>v,n\<^esub>"
+using step
+ apply cases
+ apply (frule step_z_dbm_equiv[OF prems(1)])
+ apply (rule equiv)
+ apply clarify
+ apply (drule regions.norm_FW_equiv[rotated 3])
+   prefer 4
+   apply force
+using step_z_valid_dbm[OF _ prems] valid by (simp add: valid_dbm.simps)+
+
+end (* End of context for fixed location *)
+
 subsection \<open>Multi Step\<close>
 
 declare steps_z_norm.intros[intro]
 
 lemma steps_z_norm_induct[case_names refl step, consumes 1]:
-  assumes "x1 \<turnstile> \<langle>x2, x3\<rangle> \<leadsto>\<^bsub>(k o v'),v,n\<^esub>* \<langle>x7,x8\<rangle>"
+  assumes "x1 \<turnstile> \<langle>x2, x3\<rangle> \<leadsto>\<^bsub>(\<lambda> l. k l o v'),v,n\<^esub>* \<langle>x7,x8\<rangle>"
     and "\<And>A l Z. P A l Z l Z"
     and
     "\<And>A l Z a l' Z' l'' Z'' l''' Z'''.
-        A \<turnstile> \<langle>l, Z\<rangle> \<leadsto>\<^bsub>(k o v'),v,n\<^esub>* \<langle>l',Z'\<rangle> \<Longrightarrow>
+        A \<turnstile> \<langle>l, Z\<rangle> \<leadsto>\<^bsub>(\<lambda> l. k l o v'),v,n\<^esub>* \<langle>l',Z'\<rangle> \<Longrightarrow>
         P A l Z l' Z' \<Longrightarrow>
         A \<turnstile> \<langle>l', Z'\<rangle> \<leadsto>\<^bsub>v,n,\<tau>\<^esub> \<langle>l'',Z''\<rangle> \<Longrightarrow>
-        A \<turnstile> \<langle>l'', Z''\<rangle> \<leadsto>\<^bsub>(k o v'),v,n,\<upharpoonleft>a\<^esub> \<langle>l''',Z'''\<rangle> \<Longrightarrow>
+        A \<turnstile> \<langle>l'', Z''\<rangle> \<leadsto>\<^bsub>(\<lambda> l. k l o v'),v,n,\<upharpoonleft>a\<^esub> \<langle>l''',Z'''\<rangle> \<Longrightarrow>
         P A l Z l''' Z'''"
   shows "P x1 x2 x3 x7 x8"
 using assms by (induction rule: steps_z_norm.induct) auto
@@ -362,11 +464,11 @@ next
     "A \<turnstile> \<langle>l, [D]\<^bsub>v,n\<^esub>\<rangle> \<leadsto>\<^sub>\<beta>* \<langle>l', Z\<rangle>" "[D']\<^bsub>v,n\<^esub> \<subseteq> Z"
     by auto
   from step_z_dbm_sound'[OF step(3)] have "A \<turnstile> \<langle>l', [D']\<^bsub>v,n\<^esub>\<rangle> \<leadsto>\<^bsub>\<tau>\<^esub> \<langle>l'', [D'']\<^bsub>v,n\<^esub>\<rangle>" by auto
-  from alpha_interp.step_z_mono[OF this \<open>[D']\<^bsub>v,n\<^esub> \<subseteq> Z\<close>] obtain W' where W':
+  from step_z_mono[OF this \<open>[D']\<^bsub>v,n\<^esub> \<subseteq> Z\<close>] obtain W' where W':
     "A \<turnstile> \<langle>l', Z\<rangle> \<leadsto>\<^bsub>\<tau>\<^esub> \<langle>l'', W'\<rangle>" "[D'']\<^bsub>v,n\<^esub> \<subseteq> W'"
     by auto
   from Z(1) \<open>valid_dbm D\<close>  have "Z \<subseteq> V" by (metis valid_dbm_V' steps_z_beta_V V'_V)
-  with W'(1) have "W' \<subseteq> V" by (metis alpha_interp.step_z_V)
+  with W'(1) have "W' \<subseteq> V" by (metis step_z_V)
   from steps_z_norm_valid_dbm[OF step(1,5)] have "valid_dbm D'" .
   with step_z_norm_valid_dbm'[OF step(4)] step_z_valid_dbm'[OF step(3)] have
     "valid_dbm D''" "valid_dbm D'''"
@@ -396,8 +498,6 @@ proof -
   from assms have "[D]\<^bsub>v,n\<^esub> \<subseteq> V" by (metis valid_dbm_V' V'_V)
   from steps_z_alpha_sound'[OF Z(1) this] Z(2) assms(3) show ?thesis by auto
 qed
-
-print_statement steps_z.induct
 
 lemmas norm_beta_complete' = norm_beta_complete[OF _ gcn va]
 lemmas step_z_dbm_DBM' = step_z_dbm_DBM[OF _ gcn]
@@ -444,7 +544,9 @@ proof (induction A \<equiv> A l Z _ _ arbitrary: D)
   then show ?case by blast
 next
   case (step l Z l' Z' a l'' Z'' l''' Z''')
-  from alpha_interp.step_z_mono[OF step(1,6)] obtain W' where W':
+  interpret regions: Regions_global _ _ _ "k l''"
+    by standard (rule finite clock_numbering not_in_X non_empty)+
+  from step_z_mono[OF step(1,6)] obtain W' where W':
     "A \<turnstile> \<langle>l, [D]\<^bsub>v,n\<^esub>\<rangle> \<leadsto>\<^bsub>\<tau>\<^esub> \<langle>l', W'\<rangle>" "Z' \<subseteq> W'"
     by blast
   from step_z_dbm_DBM'[OF this(1)] obtain D' where D':
@@ -452,14 +554,14 @@ next
     by blast
   have "valid_dbm D'"
     using D'(1) step.prems(1) step_z_valid_dbm' by auto
-  from alpha_interp.step_z_mono[OF step(2) \<open>Z' \<subseteq> W'\<close>] obtain W'' where
+  from step_z_mono[OF step(2) \<open>Z' \<subseteq> W'\<close>] obtain W'' where
     "A \<turnstile> \<langle>l', W'\<rangle> \<leadsto>\<^bsub>\<upharpoonleft>a\<^esub> \<langle>l'', W''\<rangle>" "Z'' \<subseteq> W''"
     by blast
-  then have "A \<turnstile> \<langle>l', [D']\<^bsub>v,n\<^esub>\<rangle> \<leadsto>\<^bsub>\<beta>(\<upharpoonleft>a)\<^esub> \<langle>l'', Approx\<^sub>\<beta> W''\<rangle>" unfolding \<open>W' = _\<close> by auto
+  then have "A \<turnstile> \<langle>l', [D']\<^bsub>v,n\<^esub>\<rangle> \<leadsto>\<^bsub>\<beta>(\<upharpoonleft>a)\<^esub> \<langle>l'', Approx\<^sub>\<beta> l'' W''\<rangle>" unfolding \<open>W' = _\<close> by auto
   from norm_beta_complete'[OF this \<open>valid_dbm D'\<close>] obtain D'' where D'':
-    "A \<turnstile> \<langle>l', D'\<rangle> \<leadsto>\<^bsub>\<N>\<upharpoonleft>a\<^esub> \<langle>l'', D''\<rangle>" "[D'']\<^bsub>v,n\<^esub> = Approx\<^sub>\<beta> W''" "valid_dbm D''"
+    "A \<turnstile> \<langle>l', D'\<rangle> \<leadsto>\<^bsub>\<N>\<upharpoonleft>a\<^esub> \<langle>l'', D''\<rangle>" "[D'']\<^bsub>v,n\<^esub> = Approx\<^sub>\<beta> l'' W''" "valid_dbm D''"
     by auto
-  from beta_interp.apx_subset this(2) \<open>Z'' \<subseteq> _\<close> have "Z'' \<subseteq> [D'']\<^bsub>v,n\<^esub>" by auto
+  from regions.beta_interp.apx_subset this(2) \<open>Z'' \<subseteq> W''\<close> have "Z'' \<subseteq> [D'']\<^bsub>v,n\<^esub>" by auto
   from step(4)[OF D''(3) this] obtain D''' where
     "A \<turnstile> \<langle>l'', D''\<rangle> \<leadsto>\<^sub>\<N>* \<langle>l''', D'''\<rangle>" "Z''' \<subseteq> [D''']\<^bsub>v,n\<^esub>"
     by blast
@@ -625,66 +727,6 @@ proof safe
   qed
 qed
 
-context Regions
-begin
-
-lemma norm_FW_equiv:
-  assumes valid: "dbm_int D n" "dbm_int M n" "[D]\<^bsub>v,n\<^esub> \<subseteq> V"
-      and equiv: "[D]\<^bsub>v,n\<^esub> = [M]\<^bsub>v,n\<^esub>"
-  shows "[norm (FW D n) (k o v') n]\<^bsub>v,n\<^esub> = [norm (FW M n) (k o v') n]\<^bsub>v,n\<^esub>"
-proof (cases "[D]\<^bsub>v,n\<^esub> = {}")
-  case False
-  with equiv fw_shortest local.non_empty_cycle_free FW_zone_equiv_spec have
-    "canonical (FW D n) n" "canonical (FW M n) n" "[FW D n]\<^bsub>v,n\<^esub> = [D]\<^bsub>v,n\<^esub>" "[FW M n]\<^bsub>v,n\<^esub> = [M]\<^bsub>v,n\<^esub>"
-  by blast+
-  with valid equiv show ?thesis
-   apply -
-   apply (subst beta_interp.apx_norm_eq[symmetric])
-   prefer 4
-   apply (subst beta_interp.apx_norm_eq[symmetric])
-  by (simp add: FW_int_preservation)+
-next
-  case True
-  show ?thesis
-   apply (subst norm_FW_empty)
-   prefer 3
-   apply (subst norm_FW_empty)
-  using valid equiv True by blast+
-qed
-
-(* XXX Maybe move *)
-lemma step_z_norm_mono:
-  assumes "A \<turnstile> \<langle>l,D\<rangle> \<leadsto>\<^bsub>\<N>(a)\<^esub> \<langle>l',D'\<rangle>" "global_clock_numbering A v n" "valid_abstraction A X k"
-  and     "valid_dbm D" "valid_dbm M"
-  and "[D]\<^bsub>v,n\<^esub> \<subseteq> [M]\<^bsub>v,n\<^esub>"
-  shows "\<exists> M'. A \<turnstile> \<langle>l, M\<rangle> \<leadsto>\<^bsub>\<N>(a)\<^esub> \<langle>l', M'\<rangle> \<and> [D']\<^bsub>v,n\<^esub> \<subseteq> [M']\<^bsub>v,n\<^esub>"
-proof -
-  from norm_beta_sound[OF assms(1,2,3,4)] have "A \<turnstile> \<langle>l, [D]\<^bsub>v,n\<^esub>\<rangle> \<leadsto>\<^bsub>\<beta>(a)\<^esub> \<langle>l', [D']\<^bsub>v,n\<^esub>\<rangle>" .
-  from step_z_beta_mono[OF this assms(6)] assms(5) obtain Z where
-    "A \<turnstile> \<langle>l, [M]\<^bsub>v,n\<^esub>\<rangle> \<leadsto>\<^bsub>\<beta>(a)\<^esub> \<langle>l', Z\<rangle>" "[D']\<^bsub>v,n\<^esub> \<subseteq> Z"
-  by auto
-  with norm_beta_complete[OF this(1) assms(2,3,5)] show ?thesis by metis
-qed
-
-lemma step_z_norm_equiv:
-  assumes step: "A \<turnstile> \<langle>l,D\<rangle> \<leadsto>\<^bsub>\<N>(a)\<^esub> \<langle>l',D'\<rangle>"
-      and prems: "global_clock_numbering A v n" "valid_abstraction A X k"
-      and valid: "valid_dbm D" "valid_dbm M"
-      and equiv: "[D]\<^bsub>v,n\<^esub> = [M]\<^bsub>v,n\<^esub>"
-  shows "\<exists> M'. A \<turnstile> \<langle>l, M\<rangle> \<leadsto>\<^bsub>\<N>(a)\<^esub> \<langle>l', M'\<rangle> \<and> [D']\<^bsub>v,n\<^esub> = [M']\<^bsub>v,n\<^esub>"
-using step
- apply cases
- apply (frule step_z_dbm_equiv[OF prems(1)])
- apply (rule equiv)
- apply clarify
- apply (drule norm_FW_equiv[rotated 3])
- prefer 4
- apply blast
-using step_z_valid_dbm[OF _ prems] valid by (simp add: valid_dbm.simps)+
-
-end
-
-
 section \<open>Appendix: Standard Clock Numberings for Concrete Models\<close>
 
 locale Regions' =
@@ -705,7 +747,7 @@ lemma in_X: assumes "v x \<le> n" shows "x \<in> X" using assms clock_numbering'
 
 end
 
-sublocale Regions' \<subseteq> Regions
+sublocale Regions' \<subseteq> Regions_global
 proof (unfold_locales, auto simp: finite clock_numbering' non_empty cn_weak not_in_X, goal_cases)
   case (1 x y) with inj in_X show ?case unfolding inj_on_def by auto
 next
@@ -721,29 +763,32 @@ qed
 
 (* This is for automata carrying real time annotations *)
 lemma standard_abstraction:
-  assumes "finite (clkp_set A)" "finite (collect_clkvt (trans_of A))" "\<forall>(_,m::real) \<in> clkp_set A. m \<in> \<nat>"
-  obtains k :: "'c \<Rightarrow> nat" where "valid_abstraction A (clk_set A) k"
+  assumes
+    "finite (Timed_Automata.clkp_set A)" "finite (Timed_Automata.collect_clkvt (trans_of A))"
+    "\<forall>(_,m::real) \<in> Timed_Automata.clkp_set A. m \<in> \<nat>"
+  obtains k :: "'c \<Rightarrow> nat" where "Timed_Automata.valid_abstraction A (clk_set A) k"
 proof -
   from assms have 1: "finite (clk_set A)" by auto
-  have 2: "collect_clkvt (trans_of A) \<subseteq> clk_set A" by auto
-  from assms obtain L where L: "distinct L" "set L = clkp_set A" by (meson finite_distinct_list)
-  let ?M = "\<lambda> c. {m . (c, m) \<in> clkp_set A}"
+  have 2: "Timed_Automata.collect_clkvt (trans_of A) \<subseteq> clk_set A" by auto
+  from assms obtain L where L: "distinct L" "set L = Timed_Automata.clkp_set A"
+    by (meson finite_distinct_list)
+  let ?M = "\<lambda> c. {m . (c, m) \<in> Timed_Automata.clkp_set A}"
   let ?X = "clk_set A"
   let ?m = "map_of L"
   let ?k = "\<lambda> x. if ?M x = {} then 0 else nat (floor (Max (?M x)) + 1)"
-  { fix c m assume A: "(c, m) \<in> clkp_set A"
-    from assms(1) have "finite (snd ` clkp_set A)" by auto
-    moreover have "?M c \<subseteq> (snd ` clkp_set A)" by force
+  { fix c m assume A: "(c, m) \<in> Timed_Automata.clkp_set A"
+    from assms(1) have "finite (snd ` Timed_Automata.clkp_set A)" by auto
+    moreover have "?M c \<subseteq> (snd ` Timed_Automata.clkp_set A)" by force
     ultimately have fin: "finite (?M c)" by (blast intro: finite_subset)
-    then have "Max (?M c) \<in> {m . (c, m) \<in> clkp_set A}" using Max_in A by auto
+    then have "Max (?M c) \<in> {m . (c, m) \<in> Timed_Automata.clkp_set A}" using Max_in A by auto
     with assms(3) have "Max (?M c) \<in> \<nat>" by auto
     then have "floor (Max (?M c)) = Max (?M c)" by (metis Nats_cases floor_of_nat of_int_of_nat_eq)
     with A have *: "?k c = Max (?M c) + 1"
     proof auto
       fix n :: int and x :: real
-      assume "Max {m. (c, m) \<in> clkp_set A} = real_of_int n"
+      assume "Max {m. (c, m) \<in> Timed_Automata.clkp_set A} = real_of_int n"
       then have "real_of_int (n + 1) \<in> \<nat>"
-        using \<open>Max {m. (c, m) \<in> clkp_set A} \<in> \<nat>\<close> by auto
+        using \<open>Max {m. (c, m) \<in> Timed_Automata.clkp_set A} \<in> \<nat>\<close> by auto
       then show "real (nat (n + 1)) = real_of_int n + 1"
         by (metis Nats_cases ceiling_of_int nat_int of_int_1 of_int_add of_int_of_nat_eq)
     qed
@@ -751,14 +796,15 @@ proof -
     moreover from A assms(3) have "m \<in> \<nat>" by auto
     ultimately have "m \<le> ?k c" "m \<in> \<nat>" "c \<in> clk_set A" using A * by force+
   }
-  then have "\<forall>(x, m)\<in>clkp_set A. m \<le> ?k x \<and> x \<in> clk_set A \<and> m \<in> \<nat>" by blast
-  with 1 2 have "valid_abstraction A ?X ?k" by - (standard, assumption+)
+  then have "\<forall>(x, m) \<in> Timed_Automata.clkp_set A. m \<le> ?k x \<and> x \<in> clk_set A \<and> m \<in> \<nat>" by blast
+  with 1 2 have "Timed_Automata.valid_abstraction A ?X ?k" by - (standard, assumption+)
   then show thesis ..
 qed
 
 definition
-  "finite_ta A \<equiv> finite (clkp_set A) \<and> finite (collect_clkvt (trans_of A))
-                 \<and> (\<forall>(_,m) \<in> clkp_set A. m \<in> \<nat>) \<and> clk_set A \<noteq> {} \<and> -clk_set A \<noteq> {}"
+  "finite_ta A \<equiv>
+    finite (Timed_Automata.clkp_set A) \<and> finite (Timed_Automata.collect_clkvt (trans_of A))
+  \<and> (\<forall>(_,m) \<in> Timed_Automata.clkp_set A. m \<in> \<nat>) \<and> clk_set A \<noteq> {} \<and> -clk_set A \<noteq> {}"
 
 lemma finite_ta_Regions':
   fixes A :: "('a, 'c, real, 's) ta"
@@ -779,10 +825,11 @@ lemma finite_ta_RegionsD:
   fixes A :: "('a, 'c, t, 's) ta"
   assumes "finite_ta A"
   obtains k :: "'c \<Rightarrow> nat" and v n x where
-    "Regions' (clk_set A) v n x" "valid_abstraction A (clk_set A) k" "global_clock_numbering A v n"
+    "Regions' (clk_set A) v n x" "Timed_Automata.valid_abstraction A (clk_set A) k"
+    "global_clock_numbering A v n"
 proof -
   from standard_abstraction assms obtain k :: "'c \<Rightarrow> nat" where k:
-    "valid_abstraction A (clk_set A) k"
+    "Timed_Automata.valid_abstraction A (clk_set A) k"
   unfolding finite_ta_def by blast
   from finite_ta_Regions'[OF assms] obtain v n x where *: "Regions' (clk_set A) v n x" .
   then interpret interp: Regions' "clk_set A" k v n x .
@@ -811,7 +858,6 @@ proof -
   qed
 qed
 
-
 lemma valid_dbm_pos:
   assumes "valid_dbm M n"
   shows "[M]\<^bsub>v,n\<^esub> \<subseteq> {u. \<forall> c. v c \<le> n \<longrightarrow> u c \<ge> 0}"
@@ -820,30 +866,5 @@ using dbm_positive assms unfolding valid_dbm_def unfolding DBM_zone_repr_def by 
 lemma (in Regions') V_alt_def:
   shows "{u. \<forall> c. v c > 0 \<and> v c \<le> n \<longrightarrow> u c \<ge> 0} = V"
 unfolding V_def using clock_numbering by metis
-
-text \<open>
-  An example of obtaining concrete models from our formalizations.
-\<close>
-lemma steps_z_norm_sound_spec:
-  assumes "finite_ta A"
-  obtains k v n where
-  "A \<turnstile> \<langle>l,D\<rangle> \<leadsto>\<^bsub>k,v,n\<^esub>* \<langle>l',D'\<rangle> \<and> valid_dbm D n \<and> [D']\<^bsub>v,n\<^esub> \<noteq> {}
-  \<longrightarrow> (\<exists>Z. A \<turnstile> \<langle>l, [D]\<^bsub>v,n\<^esub>\<rangle> \<leadsto>* \<langle>l',Z\<rangle> \<and> Z \<noteq> {})"
-proof -
-  from finite_ta_RegionsD[OF assms(1)] obtain k :: "'b \<Rightarrow> nat" and v n x where *:
-    "Regions' (clk_set A) v n x" "valid_abstraction A (clk_set A) k" "global_clock_numbering A v n"
-  .
-  from this(1) interpret interp: Regions' "clk_set A" k v n x .
-  def v' \<equiv> "\<lambda> i. if 0 < i \<and> i \<le> n then (THE c. c \<in> clk_set A \<and> v c = i) else x"
-  { fix l D l' D'
-    assume step: "A \<turnstile> \<langle>l,D\<rangle> \<leadsto>\<^bsub>(k o v'),v,n\<^esub>* \<langle>l',D'\<rangle>"
-    and valid: "valid_dbm D n" and non_empty: "[D']\<^bsub>v,n\<^esub> \<noteq> {}"
-    from valid_dbm_pos[OF valid] interp.V_alt_def have "[D]\<^bsub>v,n\<^esub> \<subseteq> interp.V" by blast
-    with valid have valid: "interp.valid_dbm D" unfolding valid_dbm_def by auto
-    from step have "interp.steps_z_norm' A l D l' D'" unfolding v'_def interp.beta_interp.v'_def .
-    note this = interp.steps_z_norm_sound''[OF *(3,2) this valid non_empty]
-  }
-  then show thesis by (blast intro: that)
-qed
 
 end
